---
layout: note
type: note
title: MATH1342 Calculus 2 for Science and Engineering
date: 2021-05-09
status: In Progress
professor: Edgar Karapetian
labels:
  - MATH1342
  - Calculus
---

# The Class

5 quizzes (lowest one dropped)

2 midterms

# Integration 

There are two methods. Don't think of them as rules.

There are infinitely many integrals that cannot be integrated. For example $\int \frac{e^x}{x} dx$ and $\int \frac{x}{\ln x} dx$.

## Substation 

Example:

$\int \frac{\ln x}{x} dx$

Let $z = \ln x$ 

Then $dz = \frac{1}{x} dx$ 

$\int z dz = \frac{z^2}{2} = \frac{1}{2} \ln (x)^2 + C$

<div class="note-block">
<strong class="note-block">NOTE: The difference between differential and derivative</strong>

$(x^2) \prime = 2x$

$\prime$ is the same thing as $\frac{d}{dx}$

Derivative: $\frac{d}{dx} \left( x^2 \right) = \frac{d (x^2)}{dx} = 2x$

Differential: $d(x^2) = 2x dx$

</div>

Example:

$\int \frac{dx}{x-1}$ 

Let $u = x-1$

$du = dx$ 

$\int \frac{du}{u} = \ln u + C = \ln (x-1) + C$

<div class="note-block">
<strong class="note-block">NOTE:</strong>

$d(x \pm C) = dx$ 

$d(2x) = 2 dx$
</div>

Example:

$\int \frac{dx}{2x+1}$

$\frac{1}{2} \int \frac{d(2x)}{2x+1}$

Example:

$\int \frac{dx}{\sqrt{2x+1} } dx$

Let $2x+1 = u$

$du = 2 dx \implies dx = \frac{1}{2} du$

$\frac{1}{2} \int \frac{du}{\sqrt{u} } = \frac{1}{2} \frac{u^{\frac{1}{2}}}{\frac{1}{2}} = \sqrt{2x + 1}  + C$

Example:

$\int \frac{\sin^{-1} x}{\sqrt{1-x^2} } dx$ 

Let $\sin ^{-1} x = u$ 

$du = \frac{dx}{\sqrt{1+ x^2} }$
 
$\int d du = \frac{u^2}{2} = \frac{\sin ^{-1} x ^2}{2} + C$

<div class="note-block">
<strong class="note-block">How to Remember Derivative of Inverse Trig:</strong>

**Sin**:

$(\sin^{-1})\prime = ?$ 

Let $\sin^{-1} (x) = z$. So we need $z'$. 

$x = \sin z$

$\frac{d}{dx (x) = \frac{d}{dx} (\sin z)}$

$1 = \cos (z) \times z' \implies z' = \frac{1}{\cos z} \implies \frac{1}{\sqrt{1-\sin ^2 (z)} } \implies \frac{1}{\sqrt{1-x^2}}$ 

**Tangent**:

$(\tan^{-1} x)' = z \implies x = \tan z$ 

$\frac{d}{dx} x = \frac{d}{dx} \tan z \implies 1 = \sec^2 z * z' \implies z' = \frac{1}{\sec ^2 z}$ 

$= \frac{1}{1+\tan^2 z} = \frac{1}{1+x^2}$

Recall that $1 + \tan ^2 (x) = \sec ^2 (x)$

</div>


Example:

$\int \frac{tan^{-1} x}{1+x^2} dx$

Example:

$\int x^2 e^{3x^3} dx$

Let $t = 3x^3$

$dt = 9x^2 dx$ 

$x^2 dx = \frac{1}{9} dt$

$\frac{1}{9} \int e^t dt = \frac{1}{9} e^t = \frac{1}{9} e^{3x^2} + C$

## By Parts

**Definition**:
$(u v) ' = v * u' + u * v'$

$\frac{d}{dx}(u v) = v \frac{d}{dx} u + u \frac{d}{dx} v$ 

$\frac{d(uv)}{dx} = v \frac{du}{dx} + u \frac{dv}{dx}$ 

$d(uv) = v du + u dv$

$\int d (uv) = \int v du + \int u dv$ 

$uv = \int v du + \int u dv$

$\int u dv = uv - \int v du$ 

What should be $u$ and $dv$?

| L | Logarithmic Functions          |
| I | Inverse Trigonometric Function |
| A | Algebraic Functions            |
| T | Trigonometric Functions        |
| E | Exponential Functions          |

(Not a rule, but is helpful)

Example:

$\int \ln x dx$

$u = \ln x \implies du = \frac{dx}{x}$

$dv = dx \implies v =x$

$\int \ln x dx = x \ln x - \int x \frac{dx }{x} = x \ln x - \int dx = x \ln x - x + C$


Example:

$\int x \ln x dx$ 

$u = \ln x \implies du = \frac{dx}{x}$

$dv = x dx \implies v = \frac{x^2}{2}$
 
$= \frac{x^2}{2} \ln x - \frac{1}{2} \int x^2 \frac{dx}{x} = \frac{x^2}{2} \ln x - \frac{1}{2} \ln x dx = \frac{x^2}{2} \ln x - \frac{1}{2} \frac{x^2}{2} = \frac{x^2}{2} \left( \ln x - \frac{1}{2} \right) + C$

Example:

$\int x^2 e^{5x} dx$ 

$u = x^2 \implies du = 2x dx$

 $dv = e^{5x} dx \implies v = \frac{1}{5} e^{5x}$

$\int x^2 e^{5x} dx = \frac{1}{5} x^2 e^{5x} - \frac{2}{5} \int x e^{5x} dx$ 

Second round:

$u = x \implies du = dx$

$dv = e^{5x} dx \implies v = \frac{1}{5} e^{5x}$

$= \frac{1}{5} x^2 e^{5x} - \frac{2}{5}\left( \frac{1}{5}x^{5x} - \frac{1}{5}\int e^{5x} dx \right)$ 

$= \frac{1}{5} x^2 e^{5x} - \frac{2}{25}x e^{5x} + \frac{2}{125} e^{5x}$

$= \frac{1}{5} e^{5x} \left( x^2 - 2x + \frac{2}{25} \right) + C$ 

Example:

$\int x \sin x dx$

$u = x \implies du = dx$

$ dv = \sin x dx \implies v = - \cos x$ 

$\int x \sin x dx = -x \cos x + \int \cos x dx$

$= - x \cos x + \sin x + C$

<div class="note-block">
<strong class="note-block">Important Trig Substitutions</strong>

$\sqrt{q^2 + x^2} $ (tan or cotan)

$\sqrt{q^2 - x^2} $ (sin or cos)

$\sqrt{x^2 - q^2} $ (sec and csc)

Always take out the $q$.

For example: $q \sqrt{1+ \left( \frac{x}{1} \right) ^2}$
</div>

First quiz on *Wednesday*.

Example:

$\int \frac{\ln x}{x} dx$ 

$u = \ln x \implies du = \frac{dx}{x}$

$dv =\frac{dx}{x} \implies v = \ln x$

$I = \int \frac{\ln x}{x} dx = \left( \ln x \right)^2 - \int \frac{\ln x}{x} dx$ 

Solve for I

$2I = \left( \ln x \right) ^{2}$ 

$\therefore I = \frac{1}{2} \left( \ln x \right) ^2 + C$

Example:

$\int e^x \sin x dx$

$u = e^{x} \implies du = d^x dx$

$dv = \sin x dx \implies v = -\cos x$

$\int e^x \sin x dx = -ex \cos x + \int e^x \cos x dx$

Lets do this again. When you do it again, stick to your choice of u and dv (otherwise, you will be left with the $\int e^x \sin x dx = \int e^x \sin x dx$).

$u = e^x \implies du = e^x dx$

$dv = \cos x dx \implies v = \sin x dx$

$= -e^x \cos x + \left( e^x \sin x - \int e^x \sin x dx \right)$

$= e^x \sin x - e^x \cos x - \int e^x \sin x dx$

$I = e^x \sin x - e^x \cos x - I$

$\therefore I = \frac{1}{2} e^x \left( \sin x - \cos x \right) + C$

Example (on your own):

$\int e^{2x} \cos \frac{x}{3} dx$ 

Example:

$\int \frac{\ln x}{x^2} dx$

We can do this both by subtitiution and by parts

By Parts:

$u = \ln x \implies du = \frac{dx}{x}$
 
$dv = \frac{dx}{x^3} \implies v= -\frac{1}{2x^2}$ 

$\int \frac{\ln x}{x^2} dx = -\frac{1}{2x^2} \ln x + \frac{1}{2} \int \frac{dx}{x^3}$

By Substitution:

$- \int \frac{\ln \frac{1}{x}}{x^2} dx$

Let $u = \frac{1}{x} \implies du = -\frac{dx}{x^2}$

$= - \int u \ln u du$ 

You can do the rest by parts

Example:
* Do not pay attention to constants -- they are irrelevant!
* We only care about the structure

$\int x e^{x^2} dx$ By Substitution
Example:

$\int x^2 e^x dx$ By parts
Example:

$u = x^2 \implies du = 2x dx$

$dv = e^x dx \implies v = e^x$ 

Example:
$\int x^2 e^{x^2} dx$ By Parts (do on your own)

Example:
$\int t^n e^t dt$ 

$u = t^n \implies du = ut^{u-1}$ 

$dv = e^t dt \implies v = e^t$

$= t^n e^t - u \int t^{u-1} e^t dt$

This is valid for all $n \ge 0$

Example:

$\int \sin ^n x dx = \int \sin^{n-1} x \sin x dx$ 

$u = \sin^{n-1} x \implies du = \left( n-1 \right) \sin^{n-2} x * \cos x$ 

$dv = \sin x dx \implies v = - \cos x$

$=-\cos x \sin^{n-1} x + \left( n-1 \right) \int \cos ^2 x \sin ^{n-2} x dx$

$=-\cos x \sin^{n-1} x + \left( n-1 \right) \left( \int \sin ^{n-2} x dx - \int \sin^u x dx \right)$

$I =- \cos x \sin^{n-1} x + \left( u-1 \right) \int \sin^{n-2} x dx - n-1) - I$


$\left( 1+ \left( n-1 \right)  \right) I = n I =-\cos x \sin^{n-1} x + \left( n+1 \right) \int \sin^{n-2} x dx$

$I = -\frac{1}{n} \cos x \sin^{n-1} x + \frac{n-1}{n} \int \sin ^{n-2} x dx$ for all $n \ge 1$

Let's now do this the traditional way

Recall $\cos^2 + \sin^2 x = 1$ and $\cos^2 x - \sin^2 x = \cos 2x$


$\int \sin^2 x dx = \frac{1}{2} \int \left( 1-\cos(2x) \right) dx$ 

$\int \sin^2 x dx = \frac{1}{2} x -\frac{1}{4} \sin 2x + C$

Example:

$\int \frac{\cos x \sqrt{x} }{\sqrt{x} } dx$

$u = \sqrt{x}$
 
$du = \frac{1}{2\sqrt{x}}$ 
 
# Integration by Partial Fraction

$\frac{P(x)}{Q(x)}$, where both $P(x)$ and $Q(x)$ are polynomials. Such that $\deg [Q(x)] > \deg [P(x)]$ ($\deg$ means the degree)

There are four distinct cases:

**Case 1**:

$Q(x)$ is a product of distinct linear factors

$Q(x) = (x+b_1)(x+b_2) ... (x+b_u)$

Then,  $\frac{P(x)}{Q(x)} = \frac{A_1}{x+b_1} + \frac{A_2}{x+b_2} + ... + \frac{A_u}{x+b_u}$ where $A_1,\ A_2,\ ...,\ A_u$ to be found.

Example:

$\frac{x^2 + 2x - 1}{x(2x-1)(x+2)} = \frac{A}{x} + \frac{B}{2x-1} + \frac{C}{x+2}$
 
$x^2 + 2x - 1 = A(2x-1)(x+2) + Bx (x+2) + Cx(2x-1)$

And solve for  `A`, `B`, and `C`.

**Case 2**:

$Q(x)$ is a product of linear factor, some of which are repeated.

That is, $Q(x)$ has $x+b$ repeated $r$ times i.e. $\left( x+b \right) ^r$ 

Example:

$\frac{x^3 - x + 1}{(x+1)x^2 (x-1)^3} = \frac{A}{x+1}+ \frac{B}{x} + \frac{C}{x^2} + \frac{D}{x-1} + \frac{E}{(x-1)^2} + \frac{F}{(x-1)^3}$
 
**Case 3**:

$Q(x)$ contains irreducible quadratic factors (none of which are repeated). That is, $Q(x)$ has factors $ax^2+bx+c$, where $b^2-4ac <0$ (that is, we have no real roots). 

Example:

$\frac{x^3+1}{(x-2)(x^2+1)(x^2+x+4)} = \frac{A}{x-2} + \frac{Bx+C}{x^2+1} + \frac{Dx+E}{x^2+x+4}$

**Case 4**:

$Q(x)$ has some repeated irreducible quadratic factors. That is $(ax^2+bx+c)^r$.

Example:

 $\frac{x^3+x^2+1}{x(x-1)(x^2+x+1)(x^2+1)^3} = \frac{A}{x} + \frac{B}{x-1} + \frac{Cx+D}{x^2+x+1} + \frac{Ex+F}{x^2 + 1} + \frac{Gx+H}{(x^2+1)^2} + \frac{Ix+J}{(x^2+1)^3}$ 
 
 Example:
 
 $\frac{1}{x^6 - x^3}= \frac{1}{x^3(x^3-1)} = \frac{1}{x^3(x-1)(x^2+x+1)}$
 
 $= \frac{A}{x} + \frac{B}{x^2} + \frac{C}{x^3} + \frac{D}{x-1} + \frac{Ex+F}{x^2+x+1}$ 
 
 Example:
 
$\frac{1}{x+x^4} = \frac{1}{x(1-x^3)} = \frac{1}{x(1-x)(1+x+x^2)}$
 
$=\frac{A}{x} + \frac{B}{1-x} + \frac{Cx+D}{1+x+x^2}$
 
 Example:
 
$\frac{x^2+1}{(x-1)^2(2x^2+1)(3x^2+2x+1)^3}$ 
 
$= \frac{A}{x-1} + \frac{B}{(x-1)^2} + \frac{Cx+D}{2x^2+1} + \frac{Ex+F}{3x^2+2x+1} + \frac{Gx+H}{(3x^2+2x+1)^2} + \frac{Ix+J}{(3x^2+2x+1)^3}$ 
 
$\frac{x^2-1}{(x-1)(x^2+2x+2)} = \frac{A}{x-1} + \frac{Bx+C}{x^2+2x+2}$ 

Full Solution Example (#68 on handout): *Expect this kind of question on the final*

$\int \frac{10}{(x+1)(x^2+4)} dx$ 

$\frac{1}{(x+1)(x^2+4)}  = \frac{A}{x+1} + \frac{Bx+C}{x^2+4}$ 

$10 = A(x^2+4) + (x+1)(Bx+C) = Ax^2 + 4A + Bx^2 + Cx + Bx + C$

$0 = A+B \implies A=-B$
 
$0=C+B \implies C+B=0$

$10 = 4A+C \implies C-4B=10$

$A=2$

$C=-B=2$ 

$B=-2$ 

$\int \frac{2}{x+1} dx + \int \frac{-2x+2}{x^2+4} dx$ (substitution) 

$= 2 \ln (x+1) - 2 \left( \int \frac{x dx}{4+x^2}- \int \frac{dx}{4+x^2} \right)$

$= 2 \ln (x+1) - 2 \left( \int \frac{x dx}{4+x^2}- \frac{1}{4} \int \frac{dx}{1+\left( \frac{x}{2} \right) ^2} \right)$


$= 2 \ln (x+1) - \ln u + \tan^{-1} \left( \frac{x}{2} \right)$ 

$= 2 \ln (x+1) - \ln (4+x^2) + \tan ^{-1} \left( \frac{x}{2} \right) + C$

For another example, do #71 on handout.
